more gc

examples/algorithms/gc.fst
@@ -39,26 +39,76 @@ type to_abs_inj (to_abs:abs_map) =
 Note: the default inferred type infers ('a -> 'b) to to_abs
       which includes an unwanted effect
 *)
-type ptr_lifts_to (to_abs:abs_map) (ptr:mem_addr) (abs:abs_node) : Type =
+type gc_state = {
+  to_abs: abs_map;
+  color: color_map;
+  abs_fields: abs_field_map;
+  fields: field_map
+}
+
+opaque type ptr_lifts_to gc_state (ptr:mem_addr) (abs:abs_node) : Type =
   valid abs
-  /\ to_abs ptr = abs
+  /\ gc_state.to_abs ptr = abs
 
-type obj_inv (i:mem_addr) (to_abs:abs_map) (abs_fields:abs_field_map) (fields:field_map) =
-  valid (to_abs i)
-  /\ ptr_lifts_to to_abs (fields i F1) (abs_fields (to_abs i) F1)
-  /\ ptr_lifts_to to_abs (fields i F2) (abs_fields (to_abs i) F2)
+opaque type obj_inv gc_state (i:mem_addr) =
+  valid (gc_state.to_abs i)
+  /\ ptr_lifts_to gc_state (gc_state.fields i F1) (gc_state.abs_fields (gc_state.to_abs i) F1)
+  /\ ptr_lifts_to gc_state (gc_state.fields i F2) (gc_state.abs_fields (gc_state.to_abs i) F2)
 
-type gc_inv (color:color_map) (to_abs:abs_map) (abs_fields:abs_field_map) (fields:field_map) =
-  to_abs_inj to_abs
+(* Maybe derive gc_inv from mutator_inv? via some higher-orderness *)
+opaque type gc_inv gc_state =
+  to_abs_inj gc_state.to_abs
   /\ (forall (i:mem_addr).
-        obj_inv i to_abs abs_fields fields
-        /\ (color i = Black ==> color (fields i F1) <> White
-                             /\ color (fields i F2) <> White)
-        /\ not (valid (to_abs i)) <==> color i = Unalloc)
+        obj_inv gc_state i
+        /\ (gc_state.color i = Black ==> gc_state.color (gc_state.fields i F1) <> White
+                                     /\ gc_state.color (gc_state.fields i F2) <> White)
+        /\ not (valid (gc_state.to_abs i)) <==> gc_state.color i = Unalloc)
 
-type mutator_inv (color:color_map) (to_abs:abs_map) (abs_fields:abs_field_map) (fields:field_map) =
-  to_abs_inj to_abs
+opaque type mutator_inv gc_state =
+  to_abs_inj gc_state.to_abs
   /\ (forall (i:mem_addr).
-        obj_inv i to_abs abs_fields fields
-        /\ (color i = Unalloc \/ color i = White)
-        /\ not (valid (to_abs i)) <==> color i = Unalloc)
+        obj_inv gc_state i
+        /\ (gc_state.color i = Unalloc \/ gc_state.color i = White)
+        /\ not (valid (gc_state.to_abs i)) <==> gc_state.color i = Unalloc)
+
+new_effect GC_STATE = STATE_h gc_state
+kind GCPost (a:Type) = a -> gc_state -> Type
+sub_effect
+  DIV   ~> GC_STATE = fun (a:Type) (wp:PureWP a) (p:GCPost a) (gc:gc_state) -> wp (fun a -> p a gc)
+
+effect GC (a:Type) (pre:gc_state -> Type) (post: gc_state -> GCPost a) =
+       GC_STATE a
+             (fun (p:GCPost a) (gc:gc_state) ->
+                  pre gc /\ (forall a gc'. (pre gc /\ post gc a gc') ==> p a gc')) (* WP *)
+             (fun (p:GCPost a) (gc:gc_state) ->
+                  (forall a gc'. (pre gc /\ post gc a gc') ==> p a gc'))           (* WLP *)
+
+effect GCMut (res:Type) (req:gc_state -> Type) (ens:gc_state -> GCPost res) =
+       GC res (fun gc -> req gc /\ mutator_inv gc)
+              (fun gc res gc' -> ens gc res gc' /\ mutator_inv gc')
+
+assume val get : unit -> GC gc_state (fun gc -> True) (fun gc res gc' -> gc=gc' /\ res=gc')
+assume val set : g:gc_state -> GC unit (fun gc -> True) (fun _ _ gc' -> b2t(g=gc'))
+
+type init_invariant (ptr:mem_addr) (gc:gc_state) =
+  forall i. mem_lo <= i /\ i < ptr
+        ==> not(valid (gc.to_abs i))
+         /\ gc.color i = Unalloc
+
+val upd_map: #a:Type -> #b:Type -> (a -> Tot b) -> a -> b -> a -> Tot b
+let upd_map f i v = fun j -> if i=j then v else f j
+
+val aux : ptr:mem_addr -> GC unit (init_invariant ptr) (fun gc _ gc' -> mutator_inv gc' /\ to_abs_inj gc'.to_abs)
+let rec aux ptr =
+  let gc = get () in
+  let gc' = {gc with
+      color=upd_map gc.color ptr Unalloc;
+      to_abs=upd_map gc.to_abs ptr no_abs
+    } in
+  set gc';
+  if ptr + 1 < mem_hi then aux (ptr + 1)
+
+val initialize: unit -> GC unit
+    (requires (fun g -> True))
+    (ensures (fun g _ g' -> mutator_inv g' /\ to_abs_inj g'.to_abs))
+let initialize () = aux mem_lo  (* TODO: hoisting aux is super ugly ... fix! *)
